Tactics.v
@@ -3,9 +3,13 @@ Require Import Program.
 Require Import Interval.
 Require Import Assertion.
 Require Import Annotation.
+Require Import Forward.
 Require Import Coq.Arith.Arith.
 Require Import Coq.omega.Omega.
 Open Scope Z_scope.
+
+
+Require Import Coq.Program.Tactics.
 
 (* In argument initial, only precondition and program inside
   effect result (expecting other assertions are not greater
@@ -14,24 +18,41 @@ Open Scope Z_scope.
   previous iterations, which reduce repeated work to guarantee
   algorithm complexity. *)
 
-Ltac interval_analysis_solver initial :=
-  let solver initial :=
-    let initial := eval compute in initial in
-    let solver' s initial' :=
-      let initial' := eval compute in initial' in
-      match initial' with
-      | ASkip ?s' => idtac (* TODO *)
-      | AAss ?x ?a1 ?s' => idtac (* TODO *)
-      | ASeq ?A1 ?A2 => idtac (* TODO *)
-      | AIf ?b1 ?A1 ?A2 ?s' => idtac (* TODO *)
-      | AWhile ?b1 ?inv ?A ?s' => idtac (* TODO *)
-      end
-    in
-    match initial with
-    APre ?s ?initial' =>
-      refine (SVPre s initial' ltac:(solver' s initial'))
+
+
+(* Lemma forward_ass (s x a1 s' : assertion) : step_valid' s (AAss x a1 (join  s')).
+  apply SVSkip. apply le_assertion_in_assertion.
+  eapply proj1. apply join_sound.
+Qed. *)
+
+Ltac solver' initial' :=
+  show_goal;
+  let s :=
+    match goal with
+    | |- step_valid' ?s _ => eval compute in s
     end
   in
+  let initial' := eval compute in initial' in
+  lazymatch initial' with
+  | ASkip ?s' =>
+    let res := eval compute in (forward_skip s s') in
+    refine (forward_skip_valid s s' res _); reflexivity
+  | AAss ?x ?a1 ?s' =>
+    let res := eval compute in (forward_ass s x a1 s') in
+      refine (forward_ass_valid s x a1 s' res _); reflexivity (* TODO *)
+  | ASeq ?A1 ?A2 => refine (SVSeq s _ _ _ _); [solver' A1 | solver' A2]
+  | AIf ?b1 ?A1 ?A2 ?s' => idtac (* TODO *)
+  | AWhile ?b1 ?inv ?A ?s' => idtac (* TODO *)
+  end.
+
+Ltac solver initial :=
+  let initial := eval compute in initial in
+  match initial with
+  APre ?s ?initial' =>
+    refine (SVPre s _ _); solver' initial'
+  end.
+
+Ltac interval_analysis_solver initial :=
   solver initial.
 
 Fixpoint initial_annotation' (c : com) : annotation' :=
@@ -47,9 +68,33 @@ Definition initial_annotation (s : assertion) (c : com) : annotation :=
   APre s (initial_annotation' c).
 
 Ltac interval_analysis initial :=
-  refine (step_valid_valid _ ltac:(interval_analysis_solver initial)).
+  refine (step_valid_valid _ _);
+  interval_analysis_solver initial.
 
-Ltac interval_analysis0 :=
-  interval_analysis default.
+Ltac interval_analysis0 prog :=
+  interval_analysis (initial_annotation default prog).
 
 
+Definition subtract_slowly_body : com :=
+  Y ::= AMinus (AId Y) (ANum 1) ;;
+  X ::= AMinus (AId X) (ANum 1).
+
+Definition test := ltac:(interval_analysis0 subtract_slowly_body).
+(* 
+test
+
+Goal True.
+pose test. simpl in v.
+
+Definition test : step_valid _ :=
+  ltac:(interval_analysis_solver (APre (Some nil) (AAss (Id "X") (APlus (AId (Id "X")) (ANum 2)) None))).
+
+Definition test := ltac:(interval_analysis0 plus2).
+
+
+
+
+
+plus2
+Search com.
+*)
