Forward.v
@@ -1,0 +1,31 @@
+Require Import Assertion.
+Require Import Annotation.
+Require Import IntervalEval.
+
+Definition forward_skip (s s' : assertion) : assertion :=
+  join s s'.
+
+Lemma forward_skip_valid (s s' res : assertion) :
+  res = forward_skip s s' ->
+  step_valid' s (ASkip res).
+Proof.
+  intros. subst.
+  apply SVSkip. apply le_assertion_in_assertion.
+  eapply proj1. apply join_sound.
+Qed.
+
+Definition forward_ass (s : assertion) (x : id) (a1 : aexp) (s' : assertion) : assertion :=
+  join (assign s x (int_aeval (assertion_to_map s) a1)) s'.
+
+Lemma forward_ass_valid (s : assertion) (x : id) (a1 : aexp) (s' res : assertion) :
+  res = forward_ass s x a1 s' ->
+  step_valid' s (AAss x a1 res).
+Proof.
+  intros. subst.
+  apply SVAss. intros.
+  eapply le_assertion_in_assertion.
+  - eapply proj1. apply join_sound.
+  - apply assign_sound.
+    + auto.
+    + apply int_aeval_sound. auto.
+Qed.
